MoreStlc.v
@@ -1,0 +1,205 @@
+Require Import SfLib.
+
+Require Import Types.
+Require Import Smallstep.
+Require Import Stlc.
+Require Import STLCWA.
+
+
+Module STLCEXTENDED.
+
+Inductive ty : Type :=
+    | TNat : ty 
+    | TArrow : ty -> ty -> ty
+    | TProd : ty -> ty -> ty
+    | TSum : ty -> ty -> ty
+    | TUnit : ty 
+    | TList : ty -> ty.
+
+    Hint Constructors ty.
+
+Inductive tm : Type :=
+    | tvar : id -> tm
+    | tabs : id -> ty -> tm -> tm 
+    | tapp : tm -> tm -> tm
+    | tnat : nat -> tm
+    | tsucc : tm -> tm
+    | tpred : tm -> tm 
+    | tmult : tm -> tm -> tm
+    | tif0 : tm -> tm -> tm -> tm
+    | tlet : id -> tm -> tm -> tm 
+    | tpair : tm -> tm -> tm 
+    | inl : ty -> tm -> tm 
+    | inr : ty -> tm -> tm
+    | scase : tm -> id -> tm -> id -> tm -> tm
+    | unit : tm 
+    | tnil : ty -> tm 
+    | tcons : tm -> tm -> tm
+    | lcase : tm -> tm -> id -> id -> tm -> tm
+    | tfix : tm -> tm.
+
+    Hint Constructors tm.
+
+Print update.
+
+    Reserved Notation "Gamma '|=' t '\in' T" (at level 40).            
+
+
+
+Inductive has_type : Context -> tm -> ty -> Prop :=
+    | tyVar :
+        forall i T G,
+            byContext G i = Some T ->
+            G |= tvar i \in T
+    | tyAbs :
+        forall i x T G Gamma,
+            update i T Gamma |= x \in G ->
+            Gamma |= tabs i T x \in TArrow T G 
+    | tyApp :
+        forall abs arg U V G,
+            G |= abs \in TArrow U V ->
+            G |= arg \in U ->
+            G |= tapp abs arg \in V
+    | tyNat :
+        forall n G,
+            G |= tnat n \in TNat
+    | tySucc :
+        forall x G,
+            G |= x \in TNat ->
+            G |= tsucc x \in TNat
+    | tyPred :
+        forall x G,
+            G |= x \in TNat ->
+            G |= tpred x \in TNat
+    | tyMult :
+        forall x y G,
+            G |= x \in TNat ->
+            G |= y \in TNat ->
+            G |= tmult x y \in TNat
+    | tyIf :
+        forall t t0 t1 G T,
+            G |= t0 \in T ->
+            G |= t1 \in T ->
+            G |= t \in TNat ->
+            G |= tif0 t t0 t1 \in T
+    | tyLet :
+        forall i x g G T U,
+            update i U G |= x \in T ->
+            G |= g \in U ->
+            G |= tlet i g x \in T
+    | tyPair :
+        forall x y U V G,
+            G |= x \in U ->
+            G |= y \in V ->
+            G |= tpair x y \in TProd U V
+    | tySum0 :
+        forall x U V G,
+            G |= x \in U ->
+            G |= inl V x \in TSum U V
+    | tySum1 :
+        forall y U V G,
+            G |= y \in V ->
+            G |= inr U y \in TSum U V
+    | tySCase :
+        forall i j matched U V lft rgt G T,
+            update i U G |= lft \in T ->
+            update j V G |= rgt \in T ->
+            G |= matched \in TSum U V ->
+            G |= scase matched i lft j rgt \in T 
+    | tyUnit :
+        forall G,
+            G |= unit \in TUnit
+    | tyNil :
+        forall G T,
+            G |= tnil T \in TList T
+    | tyCons :
+        forall x y G T,
+            G |= x \in T ->
+            G |= y \in TList T ->
+            G |= tcons x y \in TList T
+    | tyLCase :
+        forall casenil caselist matched i j T U  G,
+            G |= casenil \in U ->
+            i <> j ->
+            update i T
+                (update j (TList T) G) |= caselist \in U ->
+            G |= matched \in TList T ->
+            G |= lcase matched casenil i j caselist \in U
+    | tyFix :
+        forall x G T,
+            G |= x \in TArrow T T ->
+            G |= tfix x \in T 
+    where "Gamma '|=' t '\in' T " := (has_type Gamma t T).
+            
+
+    Hint Constructors has_type.
+
+
+Inductive value : tm -> Prop :=
+    | vnat : forall i,
+        value (tnat i)
+    | vabs : forall x T v,
+        value (tabs x T v)
+    | vprod : forall x y,
+        value x ->
+        value y ->
+        value (tpair x y)
+    | vsum0 : forall x T,
+        value x ->
+        value (inl T x)
+    | vsum1 : forall x T,
+        value x ->
+        value (inr T x)
+    | vunit :
+        value unit
+    | vnil :
+        forall T,
+        value (tnil T)
+    | vcons :
+        forall x y,
+        value x ->
+        value y ->
+        value (tcons x y)
+    | vfix :
+        forall x,
+            value x ->
+            value (tfix x).
+
+    Hint Constructors value.
+
+    Print tm.
+    
+Reserved Notation "'[' x ':=' s ']' t" (at level 20).
+Fixpoint subst (x : id) (s : tm) (org : tm) : tm :=
+    match org with
+        | tvar i => if (eq_id_dec x i) then s else org
+        | tabs t T v => tabs t T (if(eq_id_dec t x) then v else ([x := s] v))
+        | tapp a b => tapp ([x := s] a) ([x := s] b)
+        | tsucc n => tsucc ([x := s] n)
+        | tpred n => tpred ([x := s] n)
+        | tmult a b => tmult ([x := s] a) ([x := s] b)
+        | tif0 t t0 t1 => tif0 ([x := s] t) ([x := s] t0) ([x := s] t1)
+        | tlet t u v => if(eq_id_dec t x) then org else tlet t u ([x := s] v)
+        | tpair a b => tpair ([ x:= s] a) ([x := s] b)
+        | inl T v => inl T ([x := s] v)
+        | inr T v => inr T ([x := s] v)
+        | scase m ia lft ib rgt => 
+            scase ([x := s] m) ia (if (eq_id_dec ia x) then lft else [x := s] lft)
+                               ib (if (eq_id_dec ib x) then rgt else [x := s] rgt)
+        | tcons a b => tcons ([x := s] a) ([x := s] b)
+        | lcase m cn ihead itail cl =>
+            lcase ([x := s] m) ([ x:= s] cn) ihead itail
+                (if eq_id_dec ihead x then cl else 
+                    if eq_id_dec itail x then cl else [x:= s] cl)
+        | tfix v => tfix ([x := s] v)
+        | _ => org
+        end
+        where "'[' x ':=' s ']' t" := (subst x s t).
+
+
+        
+        
+
+
+
+
